\documentclass[12pt,a4paper]{article}

\usepackage{mathtools}
\usepackage{amssymb}
\usepackage{ntheorem}
\usepackage{amsmath}
\usepackage[hidelinks]{hyperref}
\usepackage{fancyhdr}
\usepackage{geometry}
\usepackage{framed}

\geometry{a4paper, left=2cm, right=2cm, bottom=2cm, top=2cm}

\pagestyle{fancy}
\fancyhead{}
\fancyhead[L]{\leftmark}
\fancyhead[R]{\rightmark}
\fancyfoot{}
\fancyfoot[C]{\thepage}
%\renewcommand{\headrulewidth}{0pt}
\renewcommand{\footrulewidth}{0pt}

\theorembodyfont{\upshape}
\theoremseparator{.}
\newcounter{nprf}[subsection]
\setcounter{nprf}{0}
\newtheorem{thm}{Theorem}[subsection]
\newtheorem{df}{Definition}[subsection]
\newtheorem{eg}{Example}[subsection]
\newtheorem{ax}{Axiom}[section]
\newtheorem{prop}{Proposition}[subsection]
\newtheorem{lem}{Lemma}[subsection]
\newtheorem{cor}{corollary}[subsection]
\newenvironment*{sol}{\par\indent\textbf{\textit{Solution. }}}{\hfill{$\square$}\par}
\newtheorem*{rmk}{\indent Remark}
\newenvironment*{prf}{\par\indent\textbf{\textit{Proof} (\stepcounter{nprf}\thenprf). }\par}{\par\hfill $\blacksquare$\par}
\newtheorem*{ext}{\indent Extension}

\linespread{1.25}

\title{Emory University\\\textbf{MATH 250 - Foundations of Mathematics Learning Notes}}
\author{Jiuru Lyu}
\date{\today}

\def\Z{{\mathbb{Z}}}
\def\R{{\mathbb{R}}}
\def\C{{\mathbb{C}}}
\def\Q{{\mathbb{Q}}}
\def\N{{\mathbb{N}}}
\def\E{{\mathbb{E}}}
\def\P{{\mathcal{P}}}
\def\d{{\mathrm{d}}}
\def\i{{\mathrm{i}}}
\def\RE{{\mathrm{Re}}}
\def\IM{{\mathrm{Im}}}
\def\Arg{{\mathrm{Arg}}}
\def\cis{\mathrm{cis}}
\def\Proj{\mathrm{Proj}}
\def\qed{\rightline{$\blacksquare$}}
\def\ddx{\frac{\d}{\d x}}
\def\dydx{\frac{\d y}{\d x}}
\def\dx{\d x}
\def\vecx{\vec{x}}
\def\vecy{\vec{y}}
\def\vecv{\vec{v}}
\def\vecw{\vec{w}}
\def\vecu{\vec{u}}
\def\veca{\vec{a}}
\def\vecb{\vec{b}}
\def\vece{\vec{e}}
\def\DNE{\mathrm{D.N.E.}}
\def\LI{\mathrm{L.I.}}
\def\st{\emph{ s.t. }}
\def\fs{\emph{ f.s. }}
\def\Iff{\emph{ iff }}
\def\WTS{\mathit{WTS}}

\begin{document}
\maketitle
\tableofcontents
\newpage

\section*{Preface}
These is my personal notes for Emory University MATH 250 Foundations of Mathematics course. 

This course requires Calculus II as pre-requisite. This course focuses on Mathematical proofs and lays foundation for any other higher level math courses, such as Real Analysis, Complex Variables, Abstract Vector Space, and Abstract Algebra. The book used for this course is \textit{An Introduction to Abstract Mathematics} by Robert Bond. 

Throughout this personal note, I use different formats to differentiate different contents, including definitions, theorems, proofs, examples, extensions, and remarks. To be more specific: 
\begin{df}[Terminology]
    This is a \textbf{definition}.	
\end{df}
\begin{thm}[Theorem Name]
    This is a \textbf{theorem}.	
\end{thm}
\begin{eg}
    This is  an \textbf{example}. 
\end{eg}

\begin{sol}
    This is the \textit{answer} part of an \textbf{example}. 
\end{sol}
\begin{rmk}
	This is a \textbf{remark} of a definition, theorem, example, or proof. 
\end{rmk}

\begin{prf}
	This is a \textbf{proof} of a theorem. 
\end{prf}
\begin{ext}
	This is a \textbf{extension} of a theorem, proof, or example. 	
\end{ext}
This is a hard course, and practice will make critical thinking, mathematical thinking, and mathematical proof skills better. Even though I put efforts into making as few flaws as possible when encoding these learning notes, some errors may still exist in this note. If you find any, please contact me via email: \url{lvjiuru@hotmail.com}. 

I hope you will find my notes helpful when developing mathematical thinking skills.

\rightline{Cheers,}
\rightline{Jiuru Lyu}

\newpage
\section{Mathematical Reasoning}
\subsection{Statement}
\begin{df}[Statement]
	A \textbf{statement} is any declarative sentence that is \underline{either true or false}.
	\begin{rmk}
		A statement cannot be ambiguous, cannot be both true and false, and cannot be sometimes true or false.
	\end{rmk}
	\begin{eg}
		Examples and Non-Examples: 
		\begin{itemize}
			\item All integers are rational numbers. -- True statement
			\item $\pi$ is irrational. -- True statement
			\item $1=0.$ -- False statement
			\item $\sqrt{2}\in\Z.$ -- False statement
			\item Every student in this class is a math major. -- False statement. (To prove this false, find a student that is not a math major.)
			\item Solve the equation $2x=3.$ -- Not a statement
			\item Chocolate chip is the best ice cream flavor. -- Not a statement
			\item $x+5=3.$ -- Not a statement. (Turn it into a statement: When $x=1$, $x+5$=3; or when $x\neq-2,\ x+5\neq3.$)
		\end{itemize}
		\begin{rmk}
			$\in$ means belongs to, and $\Z$ is the notation for integers.	
		\end{rmk}
	\end{eg}
\end{df}
\begin{rmk} 
	We denote statements by letters. 
	\begin{eg}
		$P$: ``Today is a sunny day;'' $Q$: ``$3$ is a prime number.	
	\end{eg}
	If the statement's truth depends on a variable, we include the variable in the notation.
	\begin{eg}
		$R(x)$: ``$x$ is an integer;'' $P(x)$: $x+5=3$. $P(x)$ where $x\neq-2$ is false; $P(-2)$ is true.	
	\end{eg}
	\begin{eg}
		$R(f)$: ``$f$ is an increasing function.''
		\begin{itemize}
			\item If $f(x)=e^x$, then $R(f)$ is true.
			\item If $f(x)=x^2$, then $R(f)$ is false.
		\end{itemize}	
	\end{eg}
\end{rmk}
\begin{df}[Quantifiers]
	We use the symbol $\forall$ for ``for all'' or ``for any'' and the symbol $\exists$ for ``there exists.'' $\forall$ and $\exists$ are called \textbf{quantifiers}. $\forall$ is the \textbf{universal quantifier} and $\exists$ is the \textbf{existential quantifier}.	 
	\begin{eg}
		\begin{enumerate}
			\item For any $\varepsilon>0$, there is a $\delta>0$.\[\forall\varepsilon>0,\ \exists\delta>0.\]
			\item The square of every real number is non-negative. \[\forall x\in\R,\ x^2\geq0.\]
			\item There is a real number whose square is negative. \[\exists x\in\R\st x^2<0.\]
			\item For every real number $x$, there is an integer $n$ such that $n>x$. \[\forall x\in\R,\ \exists n\in\Z\st n>x.\]
			\item For all rational numbers $x$, there exist integers $a$ and $b$ such that $x=\dfrac{a}{b}$. \[\forall x\in\Q,\ \exists a,b\in\Z\st x=\frac{a}{b}.\]
		\end{enumerate}	
	\end{eg}
	\begin{eg}
		\begin{enumerate}
			\item $\forall n\in\Z,\ \exists m\in\Z,\st m=n+5$: For every integers $n$, there exists integers $m$ such that $m=n+5$.
			\item $\forall\varepsilon>0,\ \exists\delta>0,\st\forall x,y\in\R,\text{ we have }|x-y|<\varepsilon\ \Longrightarrow\ |x^2-y^2|<\delta$: For every $\varepsilon$ greater than $0$, there exists a $\delta$ greater than $0$ such that for all real $x$ and $y$ with $|x-y|$ les than $\varepsilon$, we have $|x^2-y^2|$ is less than $\delta$. 
		\end{enumerate}
	\end{eg}
	\begin{rmk}
		$\forall\varepsilon\exists\delta$ and $\exists\delta\forall\varepsilon$ are not the same.
		
		In $\forall\varepsilon\exists\delta$, $\delta$ depends on $\varepsilon$, but $\delta$ is independent in $\exists\delta\forall\varepsilon$, meaning the same $\delta$ works for all $\varepsilon$.
		\begin{eg} 
			Compare $\forall n\in\Z,\ \exists m\in\Z\st m=n^2$ to  $\exists n\in\Z\st\forall m\in\Z,\ m=n^2.$
			\begin{sol}
				\begin{enumerate}
					\item $\forall n\in\Z,\ \exists m\in\Z\st m=n^2$: True. The square of an integer is an integer. 
					\item $\exists n\in\Z\st\forall m\in\Z,\ m=n^2.$: False: $n^2$ is just one integer and cannot be represented by all $m\in\Z$.
				\end{enumerate}
			\end{sol}
		\end{eg}
	\end{rmk}
\end{df}
\begin{df}[Negations]
	If $P$ is a statement, the \textbf{negation} of $P$, written as $\neg P$ (read as ``not $P$'' or ``negation of $P$'') is the statement ``$P$ is false.''	
	\[\begin{cases}P\text{ is true}\\\neg P\text{ is false}\end{cases}\qquad\begin{cases}P\text{ is false}\\\neg P\text{ is true}\end{cases}\]
\end{df}
\begin{eg}
	Write the negation of $P$: ``All apples are fruits'' and check the truth value of both $P$ and $\neg P$.
	\begin{sol}
		$\neg P$: Not all apples are fruits / Some apples are not fruits / There exists an apple that is not a fruit.
		
		$P$ is true and $\neg P$ is false. 
	\end{sol}
\end{eg}
\begin{eg}
	Write the negation of $P$: ``Everyday this week was hot.''
	\begin{sol}
		$\neg P$: Somedays this week were not hot. / Not all days this week were hot. / There was a day this week that was not hot. 
	\end{sol}
\end{eg}
\begin{eg}
	$P$ all primes are odd.
	
	$\neg P$: There exists ($\exists$) a prime that is even / Some primes are not odd. (True: 2 is even.)
\end{eg}
\begin{eg}
	$Q$: $\forall x\in\R,\ x^2>x$
	
	$\neg Q$: $\exists x\in\R,\st x^2\leq x$ (True: for $x=\dfrac{1}{2},\ x^2=\frac{1}{4}<x$)	
\end{eg}
\begin{eg}
	$R$: There exists a real solution to $x^2+1=0$ / $\exists x\in\R\st x^2+1=0$
	
	$\neg R$: $\forall x\in\R,\ x^2+1\neq0$ -- (True	.)
\end{eg}
\begin{rmk}[Negating Quantifiers]
	In general: 
	\[\neg(\forall x\in S, P(x))=\exists x\in S\st\neg P(x). \]
	\[\neg(\exists x\in S, P(x))=\forall x\in S, \neg P(x). \]	
\end{rmk}
\begin{eg}
	$\exists n>0\st\forall m>0, m<n$
	
	Negation: $\forall n>0, \exists m>0\st m\geq n.$	
\end{eg}
\begin{eg}
	For all $x\in\R$, there exists a $y\in\R$,$\st xy=1$
	
	Negation: $\exists x\in\R\st\forall y\in\R,\ xy\neq1$	
\end{eg}

\subsection{Compound Statements}
\begin{df}[Conjunction and Disjunction]
	The \textbf{conjunction} of $P$ and $Q$, denoted $P\wedge Q$	, is the statement ``Both $P$ and $Q$ are true.'' The \textbf{disjunction} of $P$ and $Q$, denoted $P\vee Q$, is the statement ``$P$ is true or $Q$ is true.''
\end{df}
\begin{eg}
	Which of the following are true statements?
	\begin{enumerate}
	\item The function $x^2$ is even and it is concave up.
		
		$P$: $x^2$ is even (True), $Q$: $x^2$ is concave up (True).
		\[\therefore P\wedge Q\text{ is true.}\]
	\item Every student in this class is a math major and a human being.
		
		$P$: Every student in this class is a math major (False), $Q$: Every student in this class is a human being (True).
		\[\therefore P\wedge Q\text{ is false.}\]
	\item Every student in this class is a math major or a human being.
		\[P\vee Q\text{ is true.}\]
	\end{enumerate}
\end{eg}
\begin{eg}
	The following inequality can be written in conjunctions or disjunctions.
	\begin{enumerate}
		\item $|x|<3$: ($-3<x<3$) Conjunction: $x>-3$ AND $x<3$
		\item $|x|>3$: Disjunction: $x<-3$ OR $x>3$	
	\end{enumerate}
\end{eg}
\begin{rmk}
	$\vee$ is \textbf{inclusive or}, meaning if both $P$ and $Q$ are true, then $P\vee Q$ is also true, as opposed to \textbf{exclusive or}, meaning ``either $P$ or $Q$ but not both.''	
\end{rmk}
\begin{df}[Truth Tables]
	\textbf{Truth tables} are a handy way to organize information. 
\end{df}
\begin{eg}
	Write the truth table for the statement form: $P\vee\neg Q$.
	\begin{sol}\begin{center}\begin{tabular}{c|c|c|c}
		$P$&$Q$&$\neg Q$&$P\vee\neg Q$\\
		\hline
		T&T&F&T\\
		T&F&T&T\\
		F&T&F&F\\
		F&F&T&T
	\end{tabular}\end{center}\end{sol}
\end{eg}
\begin{df}[Logically Equivalent]
	Suppose $P$ and $Q$ are statements. We say $P$ and $Q$ are \textbf{logically equivalent}, denoted as $P\equiv Q$, if they are either both true or both false.
	
	Note: If two statements are logically equivalent, their truth values match up line by line in a truth table. We use this techniques to prove two statements mathematically (logically) equivalent. 
\end{df}
\begin{eg}
	Proving the following using truth tables.
	\begin{enumerate}
		\item $\neg(\neg P)\equiv P.$
		\begin{sol}\begin{center}\begin{tabular}{c|c|c}
		$P$&$\neg P$&$\neg(\neg P)$\\
		\hline
		T&F&T\\
		F&T&F
		\end{tabular}\end{center}\end{sol}
		\item $P\vee Q\equiv Q\vee P.$
		\begin{sol}\begin{center}\begin{tabular}{c|c|c|c}
			$P$&$Q$&$P\vee Q$&$Q\vee P$\\
			\hline
			T&T&T&T\\
			T&F&T&T\\
			F&T&T&T\\
			F&F&F&F
		\end{tabular}\end{center}\end{sol}
		\item $\neg(P\vee Q)\equiv(\neg P)\wedge(\neg Q).$
		\begin{sol}\begin{center}\begin{tabular}{c|c|c|c|c|c|c}
			$P$&$Q$&$\neg P$&$\neg Q$&$P\vee Q$&$\neg(P\vee Q)$&$(\neg P)\wedge(\neg Q)$\\
			\hline
			T&T&F&F&T&F&F\\
			T&F&F&T&T&F&F\\
			F&T&T&F&T&F&F\\
			F&F&T&T&F&T&T
		\end{tabular}\end{center}\end{sol}
		\item $P\vee(Q\vee R)\equiv(P\vee Q)\vee R.$
		\begin{sol}\begin{center}\begin{tabular}{c|c|c|c|c|c|c}
			$P$&$Q$&$R$&$Q\vee R$&$P\vee(Q\vee R)$&$P\vee Q$&$(P\vee Q)\vee R$\\
			\hline
			T&T&T&T&T&T&T\\
			T&T&F&T&T&T&T\\
			T&F&T&T&T&T&T\\
			T&F&F&F&T&T&T\\
			F&T&T&T&T&T&T\\
			F&T&F&T&T&T&T\\
			F&F&T&T&T&T&T\\
			F&F&F&F&F&F&F
		\end{tabular}\end{center}\end{sol}
	\end{enumerate}	
\end{eg}
\begin{thm}[Negating Compound Statements]
	\[\neg(P\wedge Q)=\neg P\vee\neg Q\]	
	\[\neg(P\vee Q)=\neg P\wedge\neg Q\]
\end{thm}
\begin{eg}
	It is not true that the numbers $x$ and $y$ are both even. 
	
	$P$: $x$ is even; $Q$: $y$ is even.
	
	$\neg(P\wedge Q)$: $x$ is odd ($\neg P$) OR $y$ is odd ($\neg Q$).	
\end{eg}
\begin{eg}
	It is not true that $9$ is prime or $9$ is even. 
	
	$P$: $9$ is prime; $Q$: $9$ is even.
	
	$\neg(P\vee Q)$: $9$ is not prime ($\neg P$) AND $9$ is odd ($\neg Q$)	
\end{eg}
\begin{df}[Distributivity]
	\[P\wedge (Q\vee R)\equiv(P\wedge Q)\vee(P\wedge R)\]
	\[P\vee (Q\wedge R)\equiv(P\vee Q)\wedge(P\vee R)\]
\end{df}
\begin{rmk}
	Truth tables can balloon in size. Indeed, if you have $P_1,\cdots,P_n$ statements involved in your statement form, your truth table will contain $2^n$ rows. 
	
	Sometimes, prove logical equivalences without using truth tables by taking advantage of the logical equivalences already proven is more approachable. 
\end{rmk}
\begin{eg}
	Prove or disprove without using ruth tables.
	\begin{enumerate}
		\item $\neg(P\wedge(\neg Q))\equiv(\neg P)\vee Q.$
			\begin{prf}
				\[\begin{aligned}
					\neg(P\wedge(\neg Q))&\equiv\neg P\vee(\neg(\neg Q))\\
					&\equiv\neg P\vee Q\qquad\text{[Negation of }\neg Q\equiv Q\text{]}
				\end{aligned}\]	
			\end{prf}

		\item $P\wedge((Q\vee R)\vee S)\equiv(P\wedge Q)\vee(P\wedge R)\vee(P\wedge S).$
			\begin{prf}
				\[\begin{aligned}
					P\wedge((Q\vee R)\vee S)&\equiv (P\wedge(Q\vee R))\vee(P\wedge S)\qquad\text{[Distributivity]}\\
					&\equiv(P\wedge Q)\vee(P\wedge R)\vee(P\wedge S)\qquad\text{[Distributivity]}
				\end{aligned}\]	
			\end{prf}
		\item $P\vee((Q\wedge R)\wedge S)\equiv(P\vee Q)\wedge(P\vee R)\wedge(P\vee S).$
			\begin{prf}
				\[\begin{aligned}
					P\vee((Q\wedge R)\wedge S)&\equiv (P\vee(Q\wedge R))\wedge(P\vee S)\qquad\text{[Distributivity]}\\
					&\equiv(P\vee Q)\wedge(P\vee R)\wedge(P\vee S)\qquad\text{[Distributivity]}
				\end{aligned}\]	
			\end{prf}
	\end{enumerate}
\end{eg}
\begin{df}[Tautology]
	A statement form that is true in all possible cases (for example, regardless of the truth values of $P$ and $Q$) is called a \textbf{tautology}.	
\end{df}
\begin{df}[Contradiction]
	A statement that is false in all possible cases (for example, regardless of the truth values for $P$ and $Q$)	is called a \textbf{contradiction}.
\end{df}
\begin{eg}
	Classify each of the following as a tautology, a contradiction, or neither.
	\begin{enumerate}
		\item $P\vee\neg P$
		\begin{center}\begin{tabular}{c|c|c}
			$P$&$\neg P$&$P\vee\neg P$\\
			\hline
			T&F&T\\
			F&T&T
		\end{tabular}$\qquad\therefore$ Tautology.\end{center}
		\item $P\wedge\neg P$
		\begin{center}\begin{tabular}{c|c|c}
			$P$&$\neg P$&$P\wedge\neg P$\\
			\hline
			T&F&F\\
			F&T&F
		\end{tabular}$\qquad\therefore$ Contradiction.\end{center}
		\item $P\vee Q$
		\begin{center}\begin{tabular}{c|c|c}
			$P$&$A$&$P\vee Q$\\
			\hline
			T&T&T\\
			T&F&T\\
			F&T&T\\
			F&F&F
		\end{tabular}$\qquad\therefore$ Neither.\end{center}
	\end{enumerate} 	
\end{eg}

\subsection{Implications}
\begin{df}[Implications or Conditional Statements]
	The symbol $\Rightarrow$ means ``implies.'' So $P\Rightarrow Q$ means ``$P$ implies $Q$'' or ``If $P$, then $Q$.''
	\begin{eg}
		\begin{itemize}
			\item If this is an apple, then it is a fruit.
			\item If a function $f$ is differentiable, then it is continuous.
		\end{itemize}	
	\end{eg}
	\begin{rmk}
		In mathematics, the truth value of an implication is \textbf{not} determined by causality. That is, the statement $P\Rightarrow Q$ means that in all circumstances in which $P$ is true, $Q$ is also true.
		\begin{center}\begin{tabular}{c|c|c}
			$P$&$Q$&$P\Rightarrow Q$\\
			\hline
			T&T&T\\
			T&F&F\\
			F&T&T\\
			F&F&T
		\end{tabular}\end{center}
		The only way for $P\Rightarrow Q$ to be false is when $P$ is true but $Q$ is false. This implies that false assumptions can lead to any conclusions. 
	\end{rmk}
\end{df}
\begin{df}{Sufficient Condition and Necessary Condition}
	If $P\Rightarrow Q$ is true, then $P$ is called a \textbf{sufficient condition} for $Q$, and $Q$ is called a \textbf{necessary condition} for $P$. There are many different ways to write $P\Rightarrow Q$in English: 
	\[P\implies Q\begin{cases}\text{If }P,\ \text{then }Q.\\Q\text{ if }P.\\Q\text{ whenever }P.\\Q,\ \text{provided that }P\\\text{Whenever }P,\text{ then also }Q.\\P\text{ is a sufficient condition for }Q.\\\text{For }Q\text{, it is sufficient that }P.\\Q\text{ is a necessary condition for }P.\\\text{For }P\text{, it is necessary that }Q.\\P\text{ only if }Q.\end{cases}\]	
\end{df}
\begin{thm}[Negation of Implications]
	Negation of an implication is a conjunction:\[\neg(P\Rightarrow Q)\equiv P\wedge\neg Q\]	
\end{thm}
\begin{eg}
	Negate the following: \[\forall\varepsilon\ \exists\delta>0,\ |x-y|<\varepsilon\implies|x^2-y^2|<\delta.\]
	\begin{sol}
		\[\exists\varepsilon\st\forall\delta>0,\ |x-y|<\varepsilon\text{ and }|x^2-y^2|\geq\delta.\]
	\end{sol}
\end{eg}
\begin{eg}
	Write in symbols and negate the statement $P$: ``For any positive $\varepsilon$ there exists a positive $M$ such that $|f(x)-b|<\varepsilon$ whenever $x>M.$''	
	\begin{sol}
		\[P:\ \forall\varepsilon>0,\ \exists M>0\st x>M\implies|f(x)-b|<\varepsilon.\]\[\neg P:\ \exists\varepsilon>0\st\forall M>0,\ x>M\text{ and }|f(x)-b|\geq\varepsilon.\]	
	\end{sol}
\end{eg}
\begin{df}[Axiom]
	An \textbf{axiom} is a statement which is regarded as being established, accepted, or self-evidently true.
\end{df}
\begin{df}[Theorem]
	A \textbf{theorem} is a statement that is true and has been verified as true.	
\end{df}
\begin{df}[Proposition]
	A \textbf{proposition} is a smaller, less important theorem.	
\end{df}
\begin{df}[Lemma]
	A \textbf{lemma} is a theorem whose main purpose is to help prove another theorem.	
\end{df}
\begin{df}[Corollary]
	A \textbf{corollary} is a result that is the immediate consequence of a theorem. 	
\end{df}
\begin{rmk}[Proving a theorem]
	Want to show ($\WTS$) $P\Rightarrow Q$: If	$P$ is false, $P\Rightarrow Q$ is automatically true, so there's nothing to show here. However, if $P$ is true, we need to show $Q$ is true (for $P\Rightarrow Q$ to be true)l.
	
	First line of a direct proof: Suppose $P$.
	
	Last line of a direct proof: Therefore $Q$.
\end{rmk}
\begin{df}[Divisibility]
	Let $a$ and $b$ be integers, with $a$ non-zero. We say $a$ \textbf{divides} $b$, written $a\mid b$, if there exists an \emph{integer} $k$ such that $b=ak$.
	
	In this case, we way that $a$ is a \textbf{factor} of $b$, and that $b$ is a \textbf{multiple} of $a$.
	
	Also note that $a\nmid b$ means that $a$ does not divide $b$. That is, $\nexists k\in\Z$, such that $b=ak$.
\end{df}
\begin{df}[Even]
	Let $n$ be integer. We say $n$ is \textbf{eve} if $2\mid n$.	
\end{df}
\begin{df}[Odd]
	Let $n$ be an integer. We say $n$ is \textbf{odd} if $2\nmid n$, $n=2k+1$, or $n=2k-1$ for some ($\fs$) $k\in\Z.$	
\end{df}
\begin{ext}
	The possible remainders if we divide an integer by $5$ is $0,\ 1,\ 2,\ 3,\ 4$, so we can suppose $n$ to be $5k,\ 5k+1,\ 5k+2,\ 5k+3,\ 5k+4$, respectively. 	
\end{ext}
\begin{ax}\label{ax1.1}
	Integers are closed under addition.	
\end{ax}
\begin{ax}\label{ax1.2}
	If $k\in\Z, (-k)\in\Z$.
\end{ax}
\begin{framed}
\noindent\texttt{Let $a,\ b$ and $c$ be integers, with $a$ non-zero. If $a\mid b$ and $a\mid c$, then $a\mid (b+c).$}
\begin{prf}
	Let $a,b,c\in\Z$ with $a\neq0$.\par Suppose $a\mid b$ and $a\mid c$. Then, by definition of divides, $\exists k,l\in\Z\st$\[b=ak\qquad\text{and}\qquad c=al.\] \par Then, $b+c=ak+al=a(k+l).$\par Since $k+l\in\Z$ (Axiom \ref{ax1.1}), by definition, $a\mid(b+c).$	
\end{prf}
\end{framed}
\begin{framed}
\noindent\texttt{Let $a$ and $b$ be integers, with $a$ non-zero. If $a\mid b$, then $a\mid(-b)$ and $(-a)\mid b$.}
\begin{prf}
	Let $a,b\in\Z$, with $a\neq0$.\par Suppose $a\mid b$. Then by definition of divides, $\exists k\in\Z\st b=ak.$\par Multiple both sides of this equation by (-1): \[-b=-ak=a(-k).\]\par Since $(-k)\in\Z,$ we get $a\mid (-b)$.$\qquad[\text{Axiom}\ref{ax1.2}]$\par Multiple $-b=a(-k)$ by $(-1)$ on both sides: \[b=(-a)(-k)\]\par Since $(-k)\in\Z,$ we see that $(-a)\mid b.$
\end{prf}	
\end{framed}
\begin{framed}
\noindent\texttt{Let $a,\ b,\ $and $c$ be integers, with $a$ and $b$ non-zero. If $(ab)\mid(ac)$, then $b\mid c.$}
\begin{prf}
	Let	$a,b,c\in\Z$ with $a\neq0$ and $b\neq0$.\par Suppose $(ab)\mid(ac)$. Then $\exists k\in\Z\st ac=(ab)k$.\par Divide both sides of the equation by $a$: \[c=bk.\]\par Since $k\in\Z$, by definition of divides, $b\mid c$.
\end{prf}
\end{framed}
\begin{framed}
\noindent\texttt{Let $n$ be an integer. If $n$ is of the form $3k+1$ for some integer $k$, then $n^2$ is again of the form $4k'+1$ for some integer $k'$.}
\begin{prf}
	Let $n\in\Z$.\par Suppose $n=3k+1\fs k\in\Z$.\par Squaring both sides: \[\begin{aligned}n^2=(3k+1)^2&=9k^2+6k+1\\&=3(3k^2+2k)+1.\end{aligned}\]\par Set $k'=3k^2+2k.$\par As $k\in\Z$, $3k^2, 2k\in\Z$, $k'=3k^2+2k\in\Z$.\par Then, $n^2$ is in the form of $3k'+1\fs k'\in\Z.$
\end{prf}
\end{framed}
\begin{framed}
\noindent\texttt{Let $n$ and $m$ be integers. If $n$ and $m$ are even, then $n+m$ is even.}
\begin{prf}
	Let $n,m\in\Z$.\par Suppose $n$ and $m$ are even. Then $\exists s,t\in\Z\st$ \[n=2s\qquad\text{and}\qquad m=2t.\]\par Then\[\begin{aligned}n+m&=2s+2t\\&=2(s+t)\end{aligned}\]\par Since $(s+t)\in\Z$, by definition, $n+m$ is even.
\end{prf}
\end{framed}
\begin{framed}
\noindent\texttt{Let $n$ and $m$ be integers. If $m$ is even, then $mn$ is even.}
\begin{prf}
	Let $n,m\in\Z.$\par Suppose $m$ is even. Then $\exists k\in\Z,\st m=2k.$\par So, $mn=(2k)n=2(kn).$\par Since $(kn)\in\Z$, by definition, $mn$ is even.	
\end{prf}
\end{framed}
\begin{df}[Parity]
	If $x$ and $y$ have the same \textbf{parity}, then $x$ and $y$ both are odd or both are even. 	
\end{df}

\begin{framed}
\noindent\texttt{If $x\in\Z$, then $x$ and $x^2$ have the same parity.}
\begin{rmk} Sometimes, it is helpful to do a case analysis!\end{rmk}
\begin{prf}
	Let $x\in\Z$\par $\boxed{\text{Case }1}$ Suppose $x$ is even.\par Then, by definition, $x=2k\fs k\in\Z.$\par So, $x^2=(2k)^2=4k^2=2(2k^2)$.\par Since $(2k^2)\in\Z$, by definition, $x^2$ is even. \par $\boxed{\text{Case }2}$ Suppose $x$ is odd.\par Then, by definition, $x=2l+1\fs l\in\Z.$\par So, $x^2=(2l+1)^2=4l^2+4l+1=2(2l^2+2l)+1$\par Since $(2l^2+2l)\in\Z$, by definition, $x^2$ is odd.
\end{prf}
\end{framed}

\subsection{Contrapositive and Converse}
\begin{framed}
\noindent\texttt{Let $n$ be an integer. Prove that if $3\nmid n$, then $3\mid n^2-1.$}
\begin{prf}
	Let $n\in\Z$. Suppose $3\nmid n$.\par
	$\boxed{\text{Case }1}$ Then $n=3k+1\fs k\in\Z.$\[\begin{aligned}
		n^2-1&=(3k+1)^2-1\\&=9k^2+6k+1-1\\&=9k^2+6k\\&=3(3k^2+2k)
	\end{aligned}\]\par Since $(3k^2+2k)\in\Z$, by definition, $3\mid n^2-1.$\par 
	$\boxed{\text{Case }2}$ Then $n=3l+2\fs l\in\Z.$\[\begin{aligned}
		n^2-1&=(3l+2)^2-1\\&=9l^2+18l+4-1\\&=9l^2+18l+3\\&=3(3l^2+6l+1)
	\end{aligned}\]\par Since $(3l^2+6l+1)\in\Z$, by definition, $3\mid n^2-1.$
\end{prf}
\end{framed}
Sometimes, we can form new implications from old ones. Let $P$ and $Q$ to be statement, and consider the implication $P\Rightarrow Q.$
\begin{df}[Converse]
	The \textbf{converse} of $P\Rightarrow Q$ is the implication $Q\Rightarrow P.$	
\end{df}
\begin{df}[Contrapositive]
	The \textbf{contrapositive} of $P\Rightarrow Q$ is the implication $\neg Q\Rightarrow\neg P.$	
\end{df}
\begin{rmk} A question that we are interested in is that ``are these equivalent to the original implication?''\end{rmk}
\begin{thm}
	\[\neg Q\Rightarrow\neg P\equiv P\Rightarrow Q.\]
	\begin{center}\begin{tabular}{c|c|c|c|c|c}
		$P$&$Q$&$P\Rightarrow Q$&$\neg P$&$\neg Q$&$\neg Q\Rightarrow\neg P$\\
		\hline
		T&T&T&F&F&T\\
		T&F&F&F&T&F\\
		F&T&T&T&F&T\\
		F&F&T&T&T&T
	\end{tabular}\end{center}
\end{thm}
Since the contrapositive of an implication is logically equivalent to the original implication, we sometimes prove the contrapositive in order to prove the original statement. 
\begin{framed}
\noindent\texttt{Prove that if the product of two integers $x$ and $y$ is even, at least one of them must be even.}
\begin{prf}
	We will prove the contrapositive: ``If $x$ and $y$ are both odd, then $xy$ is odd.''\par Let $x,y\in\Z$. Suppose $x$ and $y$ are odd.\par Then $\exists k,l\in\Z\st x=2k+1\text{ and }y=2l+1.$\par So, \[\begin{aligned}
		xy=(2k+1)(2l+1)&=4kl+2k+2l+1\\&=2(2kl+k+l)+1
	\end{aligned}\]\par Since $2kl+k+l\in\Z$, we see that $xy$ is odd.
\end{prf}	
\end{framed}
\begin{framed}
\noindent\texttt{Let $x\in\Z$. Prove that if $x^2-4x+7$ is even, then $x$ is odd. }\par
Contrapositive: If $x$ is even, then $x^2-4x+7$ is odd.
\begin{prf}
	We will prove the contrapositive.\par Let $x\in\Z$. Suppose $x$ is even. Then $x=2k\fs k\in\Z$.\par Then \[\begin{aligned}
		x^2-4x+7&=(2k)^2-4(2k)+7\\&=4k^2-8k+7\\&=2(2k^2-4k+3)+1
	\end{aligned}\]\par Since $2k^2-4k+3\in\Z$, by definition, $x^2-4x+7$ is odd. 
\end{prf}
\end{framed}
\begin{framed}
\noindent\texttt{Let $n\in\Z$. Prove that if $n^2$ is even, then $n$ is even.}\par 
Contrapositive: If $n$ is odd, then $n^2$ is odd. 
\begin{rmk}	This is a special case of Proof (2), where $x=y$ and is odd.\end{rmk}
\begin{prf}
	We will prove the contrapositive.\par Let $n\in\Z$. Suppose $n$ is odd. Then $n=2k+1\fs k\in\Z.$\par Then \[\begin{aligned}
		n^2=(2k+1)^2&=4k^2+4k+1\\&=2(2k^2+2k)+1
	\end{aligned}\]\par Since $(2k^2+2k)\in\Z$, we see $n^2$ is odd. 
\end{prf}
\end{framed}
\begin{framed}
\noindent\texttt{Prove that every even number is of the form $4k$ or $4k+2$ for some $k\in\Z.$}
\begin{prf}
	We will prove the contrapositive: If $x$ is of the form $4k+1$ or $4k+3$, then $x$ is odd. \par Suppose $x\in\Z$.\par $\boxed{\text{Case }1}$ Suppose $x=4k+1\fs k\in\Z$. \par Then $x=4k+1=2(2k)+1$.\par Since $2k\in\Z$, by definition, $x$ is odd. \par $\boxed{\text{Case }2}$ Suppose $x=4k+3\fs k\in\Z.$\par Then $x=4k+3=2(2k+1)+1$\par Since $2k+1\in\Z$, by definition, $x$ is odd. 
\end{prf}
\end{framed}
\begin{framed}
\noindent\texttt{Prove that every odd number is of the form $4k+1$ or $4k+4$ for some $k\in\Z$.}
\begin{rmk}	This implication is the converse of  as the contrapositive of the previous one. Here, the implication and the converse of it is both true.\end{rmk}
\begin{prf}
	We will prove the contrapositive: If $x$ is of the form $4k$ or $4k+2$, then $x$ is even.\par Suppose $x\in\Z.$ \par $\boxed{\text{Case }1}$ Suppose $x=4k\fs k\in\Z$. \par Then $x=4k=2(2k)$.\par Since $2k\in\Z$, by definition, $x$ is even. \par $\boxed{\text{Case }2}$ Suppose $x=4k+2\fs k\in\Z.$\par Then $x=4k+=2=2(2k+1)$\par Since $2k+1\in\Z$, by definition, $x$ is even. 
\end{prf}
\end{framed}
\begin{thm}[Prove by Contradiction]
	To prove $P$, we assume $\neg P$ and show that this implies an absurd statement (like $1=0$ or $0<0$).
\end{thm}
\begin{df}[Simplest-form]
	Let $m$ and $n$ be integers, with $n$ non-zero. We say the fraction $\dfrac{m}{n}$ is in \textbf{simplest-form} if $m$ and $n$ have no common factors.	
\end{df}
\begin{df}[Rational Numbers]
	Let $x$ be a real number. The number $x$ is said to be $\textbf{rational}$ if there exists integers $m$ and $n$, with $n$ non-zero, such that $x=\dfrac{m}{n}$.	
\end{df}
\begin{ax}
	After a finite number of cancellations, any	fraction $\dfrac{m}{n}$ can be written in simplest form. 
\end{ax}
\begin{framed}
\noindent\texttt{Prove that $\sqrt{2}$ is irrational.}
\begin{prf}
	Assume for the sake of contradiction that $\sqrt{2}$ is rational. \par Then, by definition, $\exists p,q\in\Z,$ with $q\neq0\st\sqrt{2}=\dfrac{p}{q}$. We can assume that $p$ and $q$ have no common factors. \par Note that $\sqrt{2}q=p$, squaring both sides, we see that $2q^2=p^2$.\par Since $q^2\in\Z$, by definition, $p^2$ is even. From Proof (4), if $p^2$ is even, then $p$ must be even. By definition, $\exists k\in\Z\st p=2k.$\par Plugging this back to our equation: $2q^2=(2k)^2=4k^2,$ $q^2=2k^2$.\par Since $k^2\in\Z$, we see that $q^2$ is even. Again, from Proof (4), if $q^2$ is even, then $q$ is even. \par \begin{center}$\divideontimes$ This contradicts the fact that $p,q$ had no common factors.\end{center}\par So, $\sqrt{2}$ must, in fact, be irrational. 
\end{prf}	
\end{framed}
\begin{framed}
\noindent\texttt{Let $0<\alpha<1.$ Prove that $\sqrt{\alpha}>\alpha.$}
\begin{prf}
	\textbf{We will use the Proof by Contradiction.}\par 
	Suppose $0<\alpha<1.$ Assume for the sake of contradiction that $\sqrt{\alpha}<\alpha.$\par Since $\alpha,\sqrt{\alpha}>0$ and $f(x)=x^2$ is an increasing function for positive $x$, squaring both sides, we have $\alpha\leq\alpha^2.$\par So, $\alpha^2-\alpha\geq0$. Then $\alpha(\alpha-1)\geq0.$\[\begin{cases}\alpha\geq0\\\alpha-1\geq0\end{cases}\qquad\text{or}\begin{cases}\alpha\leq0\\\alpha-1\leq0\end{cases}\]\par We have $\alpha\geq1\quad\text{or}\alpha\leq0$.\par\begin{center}$\divideontimes$ This contradicts with the fact that $0<\alpha<1.$\end{center}\par So, $\sqrt{\alpha}>\alpha.$
\end{prf}	
Another way to prove is by contrapositive.
\begin{prf}
	We will prove the contrapositive: If $\sqrt{\alpha}\leq\alpha$, then $\alpha\leq0$ or $\alpha\geq1.$\par Suppose $\alpha\in\R$ and $\sqrt{\alpha}\leq\alpha$.\par As $\sqrt{\alpha}$ exists, $\alpha\geq0.$\par Since $\alpha,\sqrt{\alpha}\geq0$ and $f(x)=x^2$ is an increasing function for $x\geq0$: $\alpha\leq\alpha^2.$ \par Then $\alpha^2-\alpha\geq0$, $\alpha(\alpha-1)\geq0$.\par Since $\alpha\geq0$, $\alpha-1$ must also be greater than $0$.\par So, we have $\begin{cases}\alpha\geq0\\\alpha-1\geq0\end{cases}$\par Hence, we have $\alpha\geq1.$
\end{prf}
\end{framed}
\begin{framed}
\noindent\texttt{Prove that there are no integer solutions to the equation $x^2=4y+2.$}
\begin{prf}	
	Assume for the sake of contradiction that $\exists x,y\in\Z\st x^2=4y+2.$\[x^2=4y+2=2(2y+1)\]\par Since $2y+1\in\Z$, $x^2$ is an even number, and thus $x$ is also an even number.\par Then, $\exists k\in\Z\st x=2k.$\[\begin{aligned}\therefore x^2=(2k)^2=4k^2&=4y+1\\2k^2&=2y+1\end{aligned}\]\par $\boxed{\text{Method }1}$\par Since $k^2\in\Z,$ $2k^2$ is even. Since $y\in\Z$, $2y+1$ is odd.\par Then the equation indicates an even number equals to an odd number.\par\begin{center}$\divideontimes$ This contradicts with the fact that even numbers cannot equal to an odd number.\end{center}\par $\boxed{\text{Method }2}$ \[\begin{aligned}2k^2&=2y+1\\2(k^2-y)&=1\\k^2-y&=\frac{1}{2}\end{aligned}\]\par\begin{center}$\divideontimes$ This contradicts with the fact that since $k,y\in\Z$, so does $k^2-y.$\end{center}\par So, our assumption is wrong. There is no integer solutions for $x^2=4y+2.$
\end{prf}
\end{framed}
\begin{df}[Prime Numbers]
	A prime number is a natural number that is only divisible by $1$ and itself.
	\begin{eg}2, 3, 5, 7, 11, 13, 17, 19, ...\end{eg}
\end{df}
\begin{framed}
\noindent\texttt{Prove there are infinitely many primes}
\begin{rmk} This is a very revealing proof by contradiction. It reveals a way to find a larger prime based on the primes that we already have. \end{rmk}
\begin{prf}
	Assume for the sake of contradiction that there are exactly $n$ primes, where $n\in\N$. Let's list them as $p_1,\ p_2,\ p_3,\cdots,p_n$, where $p_1=2,\ p_2=3,\cdots,$ $p_n$ is the largest prime.\par Consider the number $q=\underbrace{p_1p_2p_3\cdots p_n}_{\text{product}}+1$. Then notice that since $p_i\geq2\forall i$, we have $q>p_n$.\par Since $q>p_n$, $q$ cannot be prime, based on our assumption.\par So, $\exists p_k\in\{p_1,\ p_2,\ \cdots,\ p_n\}\st p_k\mid q.$ Then, by definition, $q=cp_k\fs c\in\Z.$\par So, \[c=\frac{q}{p_k}=\frac{p_1p_2p_3\cdots p_n+1}{p_k}=\frac{p_1p_2p_3\cdots p_n}{p_k}+\frac{1}{p_k}\]\par Then, \[\frac{1}{p_k}=c-\frac{p_1p_2p_3\cdots p_n}{p_k}\]\par Note that since $p_k$ is one prime among $p_1,\cdots p_n,$ $\dfrac{p_1p_2p_3\cdots p_n}{p_k}\in\Z.$\par Since $c\in\Z$, then $\dfrac{1}{p_k}\in\Z$.\begin{center}$\divideontimes$ This is a contradiction because $p_k\nmid1$ as $p_k\geq2\forall k.$\end{center}\par So, there must be infinitely many primes
\end{prf}
\end{framed}
\begin{framed}
\noindent\texttt{If $n\in\Z$, then $5n^2+3n+7$ is odd.}
\begin{prf}
	Suppose $n\in\Z$.\par $\boxed{\text{Case }1}$ If $n$ is even. Then $\exists k\in\Z\st n=2k.$ \[5n^2+3n+7=5(2k)^2+3(2k)+7=20k^2+6k+7=2(10k^2+3k+3)+1\]\par\hspace{10mm}Since $10k^2+3k+3\in\Z$, $5n^2+3n+7$ is odd.\par $\boxed{\text{Case }2}$ If $n$ is odd. Then $\exists k\in\Z\st n=2k+1$.\[5n^2+3n+7=5(2k+!)^2+3(2k+1)+7=20k^2+26k+15=2(10k^2+13k+7)+1\]\par\hspace{10mm}Since $10k^2+13k+7\in\Z$, $5n^2+3n+7$ is odd.
\end{prf}
\end{framed}
\begin{df}[Equivalence]
	The prove $P\iff Q$ (equivalence or biconditional, ``if and only if'' or ``$\Iff$'')	we must prove the forward implication $P\implies Q$ and the backward implication $Q\implies P$.
\end{df}
\begin{framed}
\noindent\texttt{Prove that for $x,y\in\R$, $(x+y)^2=x^2+y^2$ if and only if $x=0$ or $y=0$.}
\begin{prf}
	($\Rightarrow$): We will show that $(x+y)^2=x^2+y^2\implies x=0$ or $y=0$.\par Suppose $x,y\in\Z\st(x+y)^2=x^2+y^2$. So we have \[x^2+y^2+2xy=x^2+y^2\]\par That is, $2xy=0$ or $xy=0$. So $x=0$ or $y=0$\par ($\Leftarrow$): We will show that $x=0$ or $y=0$ $\implies(x+y)^2=x^2+y^2$. \par Notice that the equation retains symmetry. \par Suppose $x,y\in\R$. Assume $x=0$ or $y=0$.\par Without loss of generality (WLOG), we may assume that $x=0$.\par Then, \[\begin{aligned}(x+y)^2=(0+y)^2&=y^2\\x^2+y^2=0^2+y^2&=y^2\end{aligned}\]\par So, $(x+y)^2=x^2+y^2.$
\end{prf}
\end{framed}

\newpage
\section{Sets}

\subsection{Sets and Subsets}
\begin{df}[Set, Element]
	A \textbf{set} is a collection of objects, called \textbf{elements}. A set is typically denoted by a capital letter and a set's elements are listed in $\{\}$.
	\begin{eg}
	\begin{itemize}
		\item $A=\{1,2,3\}$
		\item $F=\{1,2,3,5,8,13,...\}$ the set of Fibonacci numbers
		\item $\N=\{1,2,3,4,5,...\}$ the \textbf{natural numbers} (Does not include $0$.)
		\item $\emptyset$ the \textbf{empty set}
		\item $M=\left\{\begin{pmatrix}1&0\\0&0\end{pmatrix},\begin{pmatrix}0&1\\0&0\end{pmatrix},\begin{pmatrix}0&0\\1&0\end{pmatrix},\begin{pmatrix}0&0\\0&1\end{pmatrix}\right\}$
		\item $\{\text{Ludacris},\text{T.I.},\text{Killer Mike},\text{Big Boi},\text{Andre 3000},\text{Latto}\}$
	\end{itemize}	
	\end{eg}
\end{df}
\begin{df}
	We write $a\in A$ ($a$ is in $A$) to indicate $a$ is an element of $A$ and $a\notin A$ ($a$ is not in $A$) to indicate $a$ is not an element of $A$.	
\end{df}
\begin{df}[Cardinality]
	The \textbf{cardinality} of a set $A$ is the number of elements in $A$ and is denoted $|A|.$
\end{df}
\begin{rmk} When listing the elements of a set, each element is listed only once (for example, $\{1,1\}$ is not a set) and the order of the elements doesn't matter ($\{1,2\}=\{2,1\}$). \end{rmk}
\begin{df}[Set Builder Notation]
	We can use the set builder notation to describe a general property of the elements.
	\begin{eg}
		$\{2n\mid n\in\N\}$ is ``the set of elements of the form $2n$ such that $n$ is a natural number.''	
	\end{eg}
	\begin{rmk} We use $2\Z$ to represent $\{2k\mid k\in\Z\}.$ Similarly, we have $5\Z, 10\Z,...$\end{rmk}
\end{df}
\begin{df}[Subset]
	We say a set $A$ is a \textbf{subset} of a set $B$, denoted $A\subseteq B$, if every element of $A$ is an element of $B$ (If $a\in A$, then $a\in B$). We write $A\nsubseteq B$ if $A$ is not a subset of $B$ ($\neg(A\subseteq B)=a\in A\text{ and }a\notin B.$)
	\begin{itemize}
		\item $A\subseteq B$: ``$A$ is a subset of $B$''
		\item $B\supseteq A$: ``$B$ contains $A$''
		\item $A\subsetneq B$: ``$A$ is a proper subset of $B$'' or ``$A$ is a subset of $B$, but $A\neq B$.''
	\end{itemize}
	\begin{rmk}By definition, $A\subseteq A$ (every set is a subset of itself). \end{rmk}
	\begin{rmk}$\emptyset$ is a subset of any set.\end{rmk}
\end{df}
\begin{thm}
	A set of $n$ elements has $2^n$ subsets.
	\begin{prf}
		For every element in the set, they have two options: in the subset or out the subset. Hence, there will be in total $2^n$ subsets.	
	\end{prf}
\end{thm}

\begin{df}
	Building New Sets From Old
	\begin{itemize}
		\item \textbf{Intersection}: $A\cap B=\{x\mid x\in\ A\text{ and }x\in B\}$
		\item \textbf{Union}: $A\cup B=\{x\mid x\in A\text{ or }x\in B\}$
		\item \textbf{Difference}: $A-B=A\backslash B=\{x\mid x\in A\text{ and }x\notin B\}$
	\end{itemize}
\end{df}
\begin{thm}
	\[A\cup B=B\cup A\]	
	\[A\cap B=B\cap A\]
	\[A-B\neq B-A\]
\end{thm}
\begin{df}[Universal Set]
	A \textbf{universal set} of $A$ is a set within which $A$ exists.	
\end{df}
\begin{df}[Complement]
	The \textbf{complement} of $A$ in its universal set $U$ is $\overline{A}=A^{C}=U-A.$	
\end{df}
\begin{thm}
	\[A\cup\overline{A}=U\]
	\[A\cap\overline{A}=\emptyset\]	
	Specially, if $U$ is finite, $|U|=|A|+|\overline{A}|$
\end{thm}
\begin{thm}[De Morgan's Laws]
	\[\overline{A\cup B}=\overline{A}\cap\overline{B}\]	
	\[\overline{A\cap B}=\overline{A}\cup\overline{B}\]
\end{thm}
\textbf{Set Theoretic Proofs}: Prove $a\in A$: To prove an element belongs to a set, we must prove the element satisfies the required properties of the set. 
\begin{framed}
\noindent\texttt{Prove that $14\in\{4a+7b:\ a,b\in\Z\}$}	
\begin{prf}
	Note that $14=4(0)+7(2)$\par Since $0,2\in\Z$, by definition, $14\in\{4a+7b\mid a,b\in\Z\}.$
\end{prf}
\end{framed}
\begin{thm}
	Proving $A\subseteq B$: To prove $A\subseteq B$, we must prove that if $a\in A,$ then $a\in B.$ We can do so using any technique:
	\begin{itemize}
		\item Direct proof: Suppose $a\in A$...... Therefore, $a\in B.$
		\item Contrapositive proof: Suppose $a\notin B$...... Therefore, $a\notin A.$
		\item Contradiction: Suppose $a\in A.$ Assume for the sake of contradiction that $a\in B$......$\divideontimes$
	\end{itemize}	
\end{thm}
\begin{framed}
\noindent\texttt{Prove that for all $m,n\in\Z$, we have $\{x\in\Z: mn\mid x\}\subseteq\{x\in\Z:m\mid n\}\cap\{x\in\Z:n\mid x\}.$}	
\begin{prf}
	Let $x\in\Z\st x\in\{x\in\Z: mn\mid x\}.$ Then, $mn\mid x,$ and so $x=kmn\fs k\in\Z.$\par So, $x=m(kn),$ and since $kn\in\Z$, $x\in\{x\in\Z:m\mid x\}$.\par Also, $x=n(km),$ and since $km\in\Z$, $x\in\{x\in\Z:n\mid x\}$.\par By definition of intersection, $x\in\{x\in\Z:m\mid x\}\cap\{x\in\Z:n\mid x\}$.
\end{prf}
\end{framed}
\begin{df}[Equal]
	We say two sets $A$ and $B$ are \textbf{equal}, denoted $A=B$, if they have the same elements.
	\begin{rmk}
		$A=B\iff A\subseteq B\text{ and }B\subseteq A$	
	\end{rmk}
\end{df}
\begin{framed}
\noindent\texttt{If $A$, $B$, and $C$ are sets, prove $(A\cap B)-C=(A-C)\cap(B-C)$}
\begin{prf}
	($\subseteq$): $(A\cap B)-C\subseteq(A-C)\cap(B-C)$\par Suppose $x\in(A\cap B)-C$ ($\WTS$: $x\in(A-C)\cap(B-C)$)\par By definition of intersection, $x\in A$ and $x\in B$\par By definition of difference, $x\notin C.$\par Since $x\in A$ and $x\notin C$, $x\in A-C$. Similarly, since $x\in B$ and $x\notin C$, $x\in B-C$.\par By definition of intersection, $x\in(A-C)\cap(B-C)$\par
	($\supseteq$): $(A-C)\cap(B-C)\subseteq(A\cap B)-C$\par Let $x\in(A-C)\cap(B-C)$.\par By definition of intersection, $x\in A-C$ and $x\in B-C$.\par By definition of difference, $x\in A$, $x\notin C$ and $x\in B$, $x\notin C$.\par Since $x\in A$ and $x\in B$, $x\in(A\cap B)$\par Further since $x\notin C$, by definition of difference, $x\in(A\cap B)-C.$
\end{prf}
\end{framed}
\begin{framed}
\noindent\texttt{If $A$ and $B$ are sets, prove that $A\subseteq B$ if and only if $\overline{B}\subseteq\overline{A}$.}
\begin{prf}
	($\Rightarrow$): $A\subseteq B\implies\overline{B}\subseteq\overline{A}.$\par Suppose $A\subseteq B.$ ($\WTS$: $\overline{B}\subseteq\overline{A})$\par Suppose $x\in\overline{B}.$ ($\WTS$: $x\in\overline{A}$)\par Since $x\in\overline{B}$, then $x\notin B$. Note that since $A\subseteq B$, by definition, if $x\in A$, then $x\in B.$\par By contrapositive, $x\notin B\implies x\notin A$\par Since $x\notin B$, by assumption, $x\notin A$. That is $x\in\overline{A}.$\par ($\Leftarrow$): $\overline{B}\subseteq\overline{A}\implies A\subseteq B.$\par Suppose $\overline{B}\subseteq\overline{A}$ ($\WTS$: $A\subseteq B$)\par Suppose $x\in A$ ($\WTS$: $x\in B$)\par Since $x\in A,$ then $x\notin\overline{A}.$ Since$\overline{B}\subseteq\overline{A}$, by contrapositive, \[x\notin\overline{A}\implies x\in\overline{B}.\]\par Since $x\notin\overline{A},$ by assumption, $x\notin\overline{B}$. That is, $x\in B$.
\end{prf}	
\end{framed}

\subsection{Combining Sets}
\begin{framed}
\noindent\texttt{Prove that $A\subseteq B$ if and only if $A-B=\emptyset$.}
\begin{prf}
	($\Rightarrow$): WTS: $A\subseteq B\implies A-B=\emptyset$.\par Let $A$, $B$ be sets. Suppose $A\subseteq B.$\par Assume for the sake of contradiction that $A-B\neq\emptyset$. Then $x\in A-B$.\par By definition of set difference, $x\in A$ and $x\notin B$.\par\begin{center}$\divideontimes$ This contradicts with the fact that $A\subseteq B$, and thus \end{center}\[A\subseteq B\implies A-B=\emptyset.\]
	($\Leftarrow$): WTS: $A-B=\emptyset\implies A\subseteq B.$\par $\boxed{\text{Method }1}$ We will prove the contrapositive: $A\nsubseteq B\implies A-B\neq\emptyset$.\par Suppose $A\nsubseteq B$. Then $\exists x\in A \st x\notin B$.\par By definition of set difference, $x\in A-B,$ so $A-B\neq\emptyset$ as desired.\par $\boxed{\text{Method }2}$ Direct proof.\par Suppose $A-B=\emptyset$.\par By definition of set difference, $\forall x\in A, x\in B.$\par By definition of subsets, $A\subseteq B.$
\end{prf}	
\end{framed}
\begin{df}[Power set]
	The \textbf{power set} of $A$, denoted $\P(A)$, is the set of all subset of $A$. Therefore, $|\P(A)|=2^n$ when $|A|=n.$
\end{df}
\begin{thm}
	\[x\in\P(A)\iff x\subseteq A\]	
\end{thm}
\begin{framed}
\noindent\texttt{Let $A, B$ be sets. Prove that $\P(A)\cup\P(B)\subseteq\P(A\cup B)$}
\begin{prf}
	Let $A$, $B$ be sets.\par Suppose $X\in\P(A)\cup\P(B)$ $\big[$Notation: Capital $X$ because $X$ is a set!$\big]$\par Then, by definition of union, $X\in\P(A)$ or $X\in\P(B).$\par WLOG, suppose $X\in\P(A).$ By definition of the power set, $X\subseteq A$.\par Since $A\subseteq A\cup B$, if $X\subseteq A$, then $X\subseteq A\cup B$.\par By definition of the power set, $X\in\P(A\cup B).$\par Hence, $\P(A)\cup\P(B)\subseteq\P(A\cup B).$
\end{prf}
\end{framed}
\begin{df}[Cartesian Product]
	The \textbf{Cartesian product} of two sets $A$ and $B$, denoted $A\times B$, is the set of ordered pairs (or tuples) $(a,b)$ where $a\in A$ and $b\in B$, so \[A\times B=\{(a,b)\mid a\in A, b\in B\}\]
\end{df}
\begin{rmk} In general, $A\times B\neq B\times A.$\end{rmk}
\begin{thm}
	\[|A\times B|=|A|\times|B|\]	
\end{thm}
\begin{framed}
\noindent\texttt{Let $A$, $B$, and $C$ be sets. Prove that if $B\subseteq C,$ then $A\times B\subseteq A\times C.$}
\begin{prf}
	Let $A$, $B$, and $C$ be sets. Suppose $B\subseteq C$. WTS: $A\times B\subseteq A\times C.$\par Let $x\in A\times B$. Then $x=(a,b)$ where $a\in A$ and $b\in B.$\par Since $B\subseteq C,$ if $b\in B$, then $b\in C.$\par So, $x=(a,b)\in A\times C.$\par Hence, $A\times B\subseteq A\times C.$	
\end{prf}
\end{framed}
\begin{df}[Cartesian Power]
	For a set $A$ and $n\in\N$, the \textbf{Cartesian power} $A^n$ is the set \[A^n=A\times A\times A\times\cdots\times A=\{\underbrace{(a_1,a_2,a_3,\cdots,a_n)}_{n\text{-tuple}}\mid a_1,a_2,a_3,\cdots,a_n\in A\}.\]	
\end{df}
\begin{eg}
	Most common example: the Euclidean space: $\R^n$.	
\end{eg}
\begin{df}[Indexed Sets]
	\[\bigcup_{i=1}^nA_i=A_1\cup A_2\cup A_3\cup\cdots\cup A_n=\{x\mid x\in A_i \fs i\}\] and \[\bigcap_{i=1}^nA_i=A_1\cap A_2\cap A_3\cap\cdots\cap A_n=\{x\mid x\in A_i\ \forall i\}\] This notation also works when we don't have specified stopping point: $\displaystyle\bigcup_{i=1}A_i=\{x\mid x\in A_i\fs i\}$ and $\displaystyle \bigcap_{i=1}A_i=\{x\mid x\in A_i\ \forall i\}$
\end{df}



















\end{document}